

Core Econometrics - Endogeneity and IV

Table of Contents

1. [MT Part III: Endogeneity and IV](#)
 1. [3.1 Endogeneity](#)
 1. [Measurement Errors](#)
 2. [Omitted Variables](#)
 2. [3.2 Instrument Variables](#)
 3. [3.4.2 Local Average Treatment Effects](#)
 4. [3.5 GMM](#)

MT Part III: Endogeneity and IV

3.1 Endogeneity

Measurement Errors

Measurement Error in Y \rightsquigarrow No Problem #flashcard

- Consider an additive, zero-mean, uncorrelated with x_i measurement error in the dependent variable only:

$$y_i = y_i^* + v_i \iff y_i^* = y_i - v_i$$

- y_i is the observed value
- y_i^* is the true value
- $\mathbb{E}[v_i] = 0$ (zero mean)
- $\mathbb{E}[x_i u_i] = 0$ (important assumption)
- We estimate the model:

$$\begin{aligned} y_i &= y_i^* + u_i \\ &= x_i \beta + v_i + u_i \end{aligned}$$

- We still have $\mathbb{E}[(v_i + u_i)x_i] = 0 \implies$ OLS is consistent

Measurement Error in X \rightsquigarrow Attenuation Bias (Case of Classical Errors-in-variable Assumptions) #flashcard

- General setup:

$$x_i = x_i^* + e_i \iff x_i^* = x_i - e_i$$

- Classical Error-in-variable assumptions:
 - $\mathbb{E}[x_i^* e_i] = 0$ measurement error is uncorrelated with the true value of x_i^*
 - $\mathbb{E}[u_i e_i] = 0$ measurement error is uncorrelated with the true model error u_i
 - $\text{Var}[e_i] = \sigma_e^2$ measurement error is homoskedastic
 - $\text{Var}[x_i^*] = \sigma_{x^*}^2$ population variance of the true x_i^* exists and is finite
- SLR

$$\text{Now } \hat{\beta}_{OLS} = (X'X)^{-1}X'y^* = \frac{\sum_{i=1}^n x_i y_i^*}{\sum_{i=1}^n x_i^2} = \frac{\frac{1}{n} \sum_{i=1}^n x_i y_i^*}{\frac{1}{n} \sum_{i=1}^n x_i^2}$$

Use scalar law

Using $x_i = x_i^* + e_i$ and $y_i^* = x_i^* \beta + u_i$ together with the above assumptions, we obtain

$$\begin{aligned} \text{p} \lim_{n \rightarrow \infty} \hat{\beta}_{OLS} &= \frac{\text{p} \lim_{n \rightarrow \infty} \frac{1}{n} \sum_{i=1}^n (x_i^* + e_i)(x_i^* \beta + u_i)}{\text{p} \lim_{n \rightarrow \infty} \frac{1}{n} \sum_{i=1}^n (x_i^* + e_i)^2} \\ &= \frac{\left(\text{p} \lim_{n \rightarrow \infty} \frac{1}{n} \sum_{i=1}^n x_i^{*2} \right) \beta + \text{p} \lim_{n \rightarrow \infty} \frac{1}{n} \sum_{i=1}^n x_i^* u_i + \left(\text{p} \lim_{n \rightarrow \infty} \frac{1}{n} \sum_{i=1}^n x_i^* e_i \right) \beta + \text{p} \lim_{n \rightarrow \infty} \frac{1}{n} \sum_{i=1}^n u_i e_i}{\text{p} \lim_{n \rightarrow \infty} \frac{1}{n} \sum_{i=1}^n x_i^{*2} + 2 \text{p} \lim_{n \rightarrow \infty} \frac{1}{n} \sum_{i=1}^n x_i^* e_i + \text{p} \lim_{n \rightarrow \infty} \frac{1}{n} \sum_{i=1}^n e_i^2} \\ &= \frac{\overset{0}{\text{E}(x_i^{*2})\beta} + \overset{0}{\text{E}(x_i^* u_i)} + \overset{0}{\text{E}(x_i^* e_i)\beta} + \overset{0}{\text{E}(u_i e_i)}}{\overset{0}{\text{E}(x_i^{*2})} + 2\overset{0}{\text{E}(x_i^* e_i)} + \overset{0}{\text{E}(e_i^2)}} = \frac{\text{E}(x_i^{*2})\beta + 0 + 0 + 0}{\text{E}(x_i^{*2}) + 0 + \text{E}(e_i^2)} \\ &= \underbrace{\left(\frac{\sigma_{x^*}^2}{\sigma_{x^*}^2 + \sigma_e^2} \right)}_{< 1} \beta = \frac{\beta}{1 + (\sigma_e^2 / \sigma_{x^*}^2)} \neq \beta \quad \text{if } \sigma_e^2 > 0 \end{aligned}$$

$$\begin{aligned} \text{p} \lim_{n \rightarrow \infty} \hat{\beta}_{OLS} &= \frac{\beta}{1 + (\sigma_e^2 / \sigma_{x^*}^2)} < \beta \quad \text{for } \beta > 0 \text{ and } \sigma_e^2 > 0 \\ \text{p} \lim_{n \rightarrow \infty} \hat{\beta}_{OLS} &= \frac{\beta}{1 + (\sigma_e^2 / \sigma_{x^*}^2)} > \beta \quad \text{for } \beta < 0 \text{ and } \sigma_e^2 > 0 \end{aligned}$$

MLR

- The OLS estimator of the coefficient on the variable with ME will have attenuation bias
- The OLS estimator of other coefficients will also be biased, but with unknown directions

Omitted Variables

Omitted Variable in SLR

- True DGP:

$$y_i = x_{1i}\beta_1 + x_{2i}\beta_2 + u_i$$

with $\mathbb{E}[x_{1i}u_i] = \mathbb{E}[x_{2i}u_i] = 0$ and $\mathbb{E}[u_i] = \mathbb{E}[x_{1i}] = \mathbb{E}[x_{2i}] = 0$ for simplicity

- We omit x_{2i} and estimate:

$$y_i = x_{1i}\beta_1 + (x_{2i}\beta_2 + u_i)$$

- Result:

$$\text{plim}_{n \rightarrow \infty} \hat{\beta}_1 = \beta_1 + \beta_2 \rho_{x_1, x_2}$$

- Proof:

Since $u_i \rightarrow$ demand SLR

$$\begin{aligned} \hat{\beta}_{OLS} &= (X'X)^{-1}X'y^* = \frac{\sum_{i=1}^n x_i y_i^*}{\sum_{i=1}^n x_i^2} = \frac{\frac{1}{n} \sum_{i=1}^n x_i y_i^*}{\frac{1}{n} \sum_{i=1}^n x_i^2} \\ \text{plim}_{n \rightarrow \infty} \hat{\beta}_{OLS} &= \frac{\mathbb{E}[x_i y_i^*]}{\mathbb{E}[x_i^2]} = \frac{\mathbb{E}[(x_i^* + e_i)(x_i^* \beta + u_i)]}{\mathbb{E}[(x_i^* + e_i)^2]} \\ &= \frac{\mathbb{E}[x_i^{*2}\beta] + \mathbb{E}[x_i^* u_i] + \mathbb{E}[x_i^* e_i \beta] + \mathbb{E}[e_i u_i]}{\mathbb{E}[x_i^{*2}] + 2\mathbb{E}[x_i^* e_i] + \mathbb{E}[e_i^2]} \\ &= \frac{\beta \mathbb{E}[x_i^{*2}] + 0 + 0 + 0}{\mathbb{E}[x_i^{*2}] + 2\mathbb{E}[x_i^* e_i] + \mathbb{E}[e_i^2]} \\ &= \frac{\beta \underbrace{\mathbb{E}[x_i^{*2}]}_{\sigma_{x^*}^2}}{\underbrace{\mathbb{E}[x_i^{*2}]}_{\sigma_{x^*}^2} + \underbrace{\mathbb{E}[e_i^2]}_{\sigma_e^2}} = \frac{\beta}{1 + \frac{\sigma_e^2}{\sigma_{x^*}^2}} \neq \beta \quad \text{if } \sigma_e^2 \neq 0 \end{aligned}$$

$$\begin{cases} \text{plim}_{n \rightarrow \infty} \hat{\beta}_{OLS} < \beta & \text{if } \beta > 0 \text{ and } \sigma_e^2 \neq 0 \\ \text{plim}_{n \rightarrow \infty} \hat{\beta}_{OLS} > \beta & \text{if } \beta < 0 \text{ and } \sigma_e^2 \neq 0 \end{cases}$$

The OLS estimator of β_1 is

$$\hat{\beta}_1 = (X_1'X_1)^{-1}X_1'y$$

Substituting for $y = X_1\beta_1 + X_2\beta_2 + u$ from the true model

$$\begin{aligned}\hat{\beta}_1 &= (X_1'X_1)^{-1}X_1'(X_1\beta_1 + X_2\beta_2 + u) \\ &= \beta_1 + [(X_1'X_1)^{-1}X_1'X_2] \beta_2 + (X_1'X_1)^{-1}X_1'u \\ &= \beta_1 + \hat{\delta}\beta_2 + (X_1'X_1)^{-1}X_1'u\end{aligned}$$

where $\hat{\delta} = (X_1'X_1)^{-1}X_1'X_2$ is the OLS estimator of ...

21

...the coefficient δ in a linear projection of the omitted variable x_{2i} on the included variable x_{1i} , i.e.

$$x_{2i} = x_{1i}\delta + e_i$$

Taking probability limits, and using $E(x_{1i}u_i) = 0$, we obtain

$$\text{p} \lim_{n \rightarrow \infty} \hat{\beta}_1 = \beta_1 + (\text{p} \lim_{n \rightarrow \infty} \hat{\delta})\beta_2 = \beta_1 + \delta\beta_2$$

Omitted Variables in MLR #flashcard

• Single Omitted Variable in MLR

- Model:

$$y_i = \beta_1 + \beta_2 x_{2i} + \dots + \beta_{K-1} x_{K-1,i} + (\beta_K x_{Ki} + u_i)$$

where $E[x_{ki}u_i] = 0$ for $k = 1, \dots, K$

- Result:

$$\text{plim}_{n \rightarrow \infty} \hat{\beta}_k = \beta_k + \beta_K \rho_{x_k, x_K | x_{i \neq K}}$$

where $\rho_{x_k, x_K | x_{i \neq K}}$ is the partial correlation between x_k, x_K , which can be obtained as δ_k in the linear projection:

$$x_{Ki} = \delta_1 + \delta_2 x_{2i} + \dots + \delta_{K-1} x_{K-1,i} + v_i$$

- Proof:

Single omitted variable

$$y_i = \beta_1 + \beta_2 x_{2i} + \dots + \beta_{K-1} x_{K-1,i} + (\beta_K x_{Ki} + u_i) \quad \text{①}$$

where $E(x_{ki}u_i) = 0$ for $k = 1, \dots, K$ (and $x_{1i} = 1$ for all $i = 1, \dots, n$)

[Relation to general model: $K_1 = K - 1, K_2 = 1$]

Linear projection of omitted x_{Ki} on all the included variables

$$x_{Ki} = \delta_1 + \delta_2 x_{2i} + \dots + \delta_{K-1} x_{K-1,i} + v_i$$

s.t. $E(x_{ki}v_i) = 0$ for $k = 1, \dots, K - 1$ (by definition of linear projection)

Multiply x_{Ki} by β_K and substitute:

$$y_i = (\beta_1 + \beta_K \delta_1) + (\beta_2 + \beta_K \delta_2) x_{2i} + \dots + (\beta_{K-1} + \beta_K \delta_{K-1}) x_{K-1,i} + (u_i + \beta_K v_i)$$

29

$$y_i = (\beta_1 + \beta_K \delta_1) + (\beta_2 + \beta_K \delta_2) x_{2i} + \dots + (\beta_{K-1} + \beta_K \delta_{K-1}) x_{K-1,i} + (u_i + \beta_K v_i)$$

Now since $E[x_{ki}(u_i + \beta_K v_i)] = 0$ for $k = 1, \dots, K - 1$, we have

$$p \lim_{n \rightarrow \infty} \hat{\beta}_k = \beta_k + \beta_K \delta_k \quad \text{for } k = 1, \dots, K - 1$$

$$(\text{Or equivalently } p \lim_{n \rightarrow \infty} \hat{\beta}_k = \beta_k + (p \lim_{n \rightarrow \infty} \hat{\delta}_k) \beta_K)$$

$$x_{Ki} = \delta_1 + \delta_2 x_{2i} + \dots + \delta_{K-1} x_{K-1,i} + v_i$$

$$\beta_K x_{Ki} = \beta_K \delta_1 + \beta_K \delta_2 x_{2i} + \dots + \beta_K \delta_{K-1} x_{K-1,i} + \beta_K v_i$$

Substitute this into ①

Multiple Omitted Variable in MLR

- Model:

$$y = X_1 \beta_1 + (X_2 \beta_2 + u)$$

- We can show that:

$$p \lim_{n \rightarrow \infty} \hat{\beta}_1 = \beta_1 + (p \lim_{n \rightarrow \infty} (X_1^T X_1)^{-1} X_1^T X_2) \beta_2$$

- OLS estimators will be biased and inconsistent (unless all omitted variables are orthogonal to all included variables) but the direction is hard to predict

Simultaneity Bias #flashcard

- The dependent variable and at least one of the explanatory variables are chosen jointly as part of the same decision problem.

3.2 Instrument Variables

THE FOLLOWING IS NOT A COMPREHENSIVE SUMMARY FOR THE IV PART!

Formulas for 2SLS Estimator #flashcard

$$\begin{aligned} \hat{\beta}_{2SLS} &= (\hat{X}^T \hat{X})^{-1} \hat{X}^T y \\ &= \left(X^T \underbrace{Z(Z^T Z)^{-1} Z^T}_{P_z} X \right)^{-1} X^T \underbrace{Z(Z^T Z)^{-1} Z^T}_{P_z} y \\ &= (\hat{X}^T X)^{-1} \hat{X}^T y \\ &= (Z^T X)^{-1} Z^T y \quad (\text{only in the just-identified case}) \end{aligned}$$

2SLS as Control Function #flashcard

- Preform 1st stage projection
- Plug in 1st-stage residuals as additional variables in the main regression

2SLS as Indirect Least Square #flashcard

- When **just-identified**, 2SLS coincides with indirect least squares

- Example: we have an IV z_i for the endogenous regressor x_i

1. Run a first stage projection

$$x_i = z_i\pi + r_i$$

2. Run a reduced-form regression:

$$y_i = z_id + u_i$$

3. Divide reduced-form coefficient by 1st-stage coefficient:

$$\hat{\beta}_{\text{indirect square}} = \frac{\hat{d}}{\hat{\pi}}$$

Consistency of 2SLS #flashcard

To establish conditions under which $\hat{\beta}_{2SLS}$ is a consistent estimator of β ,

we express $\hat{\beta}_{2SLS}$ in the form

$$\begin{aligned}\hat{\beta}_{2SLS} &= (\hat{X}'X)^{-1}\hat{X}'y \quad (\text{3rd Expression}) \\ &= (\hat{X}'X)^{-1}\hat{X}'(X\beta + u) \\ &= (\hat{X}'X)^{-1}\hat{X}'X\beta + (\hat{X}'X)^{-1}\hat{X}'u \\ &= \beta + \left(\frac{\hat{X}'X}{n}\right)^{-1} \left(\frac{\hat{X}'u}{n}\right)\end{aligned}$$

Taking probability limits

$$p \lim_{n \rightarrow \infty} \hat{\beta}_{2SLS} = \beta + p \lim_{n \rightarrow \infty} \left(\frac{\hat{X}'X}{n}\right)^{-1} p \lim_{n \rightarrow \infty} \left(\frac{\hat{X}'u}{n}\right)$$

We assume the data on (y_i, x_i, z_i) are independent and identically distributed, with $E(z_i u_i) = 0$ and $E(z_i x_i) \neq 0 \Leftrightarrow \pi \neq 0$

From the Law of Large Numbers, the vector of sample means

$$\frac{1}{n} \sum_{i=1}^n z_i u_i \xrightarrow{p} E(z_i u_i) = 0$$

We can also write $\frac{1}{n} \sum_{i=1}^n z_i u_i = \frac{1}{n} (Z'u)$, so we have

$$\left(\frac{Z'u}{n}\right) \xrightarrow{p} 0$$

$\hat{\pi}$ is a consistent estimator of the coefficient vector π in the first stage linear projection, so we also have $\hat{\pi} \xrightarrow{p} \pi \neq 0$

Since $\hat{X} = Z\hat{\pi}$, we can express

$$\left(\frac{\hat{X}'u}{n}\right) = \left(\frac{(Z\hat{\pi})'u}{n}\right) = \left(\frac{(\hat{\pi}'Z')u}{n}\right) = \hat{\pi}' \left(\frac{Z'u}{n}\right)$$

Then using Slutsky's theorem, we have

$$p \lim_{n \rightarrow \infty} \left(\frac{\hat{X}'u}{n}\right) = \pi'0 = 0$$

Similarly, from the Law of Large Numbers, the vector of sample means

$$\frac{1}{n} \sum_{i=1}^n z_i x_i \xrightarrow{p} E(z_i x_i) = M_{ZX} \neq 0$$

where $M_{ZX} = E(z_i x_i)$ is an $L \times 1$ column vector

We can also write $\frac{1}{n} \sum_{i=1}^n z_i x_i = \frac{1}{n} (Z'X)$, so we have

$$\left(\frac{Z'X}{n}\right) \xrightarrow{p} M_{ZX} \neq 0$$

Since $\hat{X} = Z\hat{\pi}$, we can express

$$\left(\frac{\hat{X}'X}{n}\right) = \left(\frac{(Z\hat{\pi})'X}{n}\right) = \left(\frac{(\hat{\pi}'Z')X}{n}\right) = \hat{\pi}' \left(\frac{Z'X}{n}\right)$$

Then using Slutsky's theorem, we have

$$p \lim_{n \rightarrow \infty} \left(\frac{\hat{X}'X}{n}\right) = \pi' M_{ZX} \neq 0$$

and

$$p \lim_{n \rightarrow \infty} \left(\frac{\hat{X}'X}{n}\right)^{-1} = (\pi' M_{ZX})^{-1} \text{ is finite}$$

$$\begin{aligned}\hat{\beta}_{2SLS} &= (\hat{X}'X)^{-1}\hat{X}'y \\ &= (\hat{X}'X)^{-1}\hat{X}'(X\beta + u) \\ &= (\hat{X}'X)^{-1}\hat{X}'X\beta + (\hat{X}'X)^{-1}\hat{X}'u \\ &= \beta + \left(\frac{\hat{X}'X}{n}\right)^{-1} \left(\frac{\hat{X}'u}{n}\right) \\ p \lim_{n \rightarrow \infty} \hat{\beta}_{2SLS} &= \beta + p \lim_{n \rightarrow \infty} \left(\frac{\hat{X}'X}{n}\right)^{-1} p \lim_{n \rightarrow \infty} \left(\frac{\hat{X}'u}{n}\right) \\ &\quad \left(\text{show this is } 0\right) \\ \frac{\hat{X}'u}{n} &= \frac{(Z\hat{\pi})'u}{n} = \frac{\hat{\pi}'Z'u}{n} = \hat{\pi}' \frac{Z'u}{n} \\ p \lim_{n \rightarrow \infty} \left(\frac{\hat{X}'u}{n}\right) &= p \lim_{n \rightarrow \infty} \left(\hat{\pi}' \frac{Z'u}{n}\right) = p \lim_{n \rightarrow \infty} \hat{\pi}' p \lim_{n \rightarrow \infty} \left(\frac{Z'u}{n}\right) = \pi' \underbrace{E[Z'u_i]}_{=0 \text{ by Kolydy assumption}} = \pi' \times 0 = 0 \\ &\quad \left(\text{show this is finite}\right) \\ \frac{\hat{X}'X}{n} &= \frac{(Z\hat{\pi})'X}{n} = \frac{\hat{\pi}'Z'X}{n} = \hat{\pi}' \left(\frac{Z'X}{n}\right) \\ p \lim_{n \rightarrow \infty} \left(\frac{\hat{X}'X}{n}\right) &= \pi' p \lim_{n \rightarrow \infty} \left(\frac{Z'X}{n}\right) = \pi' \underbrace{E[Z_i X_i]}_{\neq 0 \text{ by Identification Assumption}} = \pi' M_{ZX} \neq 0 \\ \Rightarrow p \lim_{n \rightarrow \infty} \hat{\beta}_{2SLS} &= \beta + (\pi' M_{ZX})^{-1} \times 0 = \beta \quad \square\end{aligned}$$

Now recalling that

$$p \lim_{n \rightarrow \infty} \hat{\beta}_{2SLS} = \beta + p \lim_{n \rightarrow \infty} \left(\frac{\hat{X}'X}{n} \right)^{-1} p \lim_{n \rightarrow \infty} \left(\frac{\hat{X}'u}{n} \right)$$

we have shown:

- i) $p \lim_{n \rightarrow \infty} \left(\frac{\hat{X}'u}{n} \right) = 0$, given the instrument validity condition $E(z_i u_i) = 0$
- ii) $p \lim_{n \rightarrow \infty} \left(\frac{\hat{X}'X}{n} \right)^{-1}$ exists and is finite, given the instrument informativeness condition $E(z_i x_i) \neq 0 \leftrightarrow \pi \neq 0$

Given these two properties of the instrumental variables in z_i , we obtain the consistency result

$$p \lim_{n \rightarrow \infty} \hat{\beta}_{2SLS} = \beta \quad \text{or} \quad \hat{\beta}_{2SLS} \xrightarrow{p} \beta$$

2SLS as GMM #flashcard

- GMM tries to best match the sample analogue of population moment $E[z_i u_i] = 0$
- Just identified case: $\hat{\beta}_{GMM} = \hat{\beta}_{2SLS}$
- Over-identified case: the GMM estimator minimises a weighted quadratic distance:

$$\begin{aligned} \hat{\beta}_{GMM} &= \arg \min_{\beta} \{u^T Z W_n Z^T u\} \\ &= \arg \min_{\beta} \left\{ \left(\frac{1}{n} \sum_{i=1}^n u_i(\beta) z_i^T \right) W_n \left(\frac{1}{n} \sum_{i=1}^n u_i(\beta)^T z_i \right) \right\} \end{aligned}$$

- 2SLS uses a particular weight matrix $W_{2SLS} = (Z^T Z)^{-1}$, which is the most efficient one under homoskedasticity

Inference and Var Estimation for 2SLS #flashcard

- Assumptions: Validity + Informative
- Large-sample distribution:

$$\hat{\beta}_{2SLS} \sim^a N \left(\beta, \frac{V}{n} \right)$$

- Under homoskedasticity ($E[u_i^2 | z_i] = \sigma^2$), the consistent estimator for estimation variance is:

$$\widehat{Var}(\hat{\beta}_{2SLS}) = \frac{\hat{V}}{n} = \hat{\sigma}^2 (\hat{X}^T \hat{X})^{-1}$$

where $\hat{\sigma}^2 = \frac{1}{n} \sum_{i=1}^n \hat{u}_i^2$

- Thus:

$$\hat{\beta}_{2SLS} \sim^a N \left(\beta, \hat{\sigma}^2 (\hat{X}^T \hat{X})^{-1} \right)$$

- Under heteroskedasticity, there is a HR estimator:

$$\widehat{Var}_{HR}(\hat{\beta}_{2SLS}) = \frac{\hat{V}_{HR}}{n} = (\hat{X}^T \hat{X})^{-1} \left(\sum_{i=1}^n \hat{u}_i^2 \hat{x}_i \hat{x}_i^T \right) (\hat{X}^T \hat{X})^{-1}$$

- Thus:

$$\hat{\beta}_{2SLS} \sim^a N \left(\beta, (\hat{X}^T \hat{X})^{-1} \left(\sum_{i=1}^n \hat{u}_i^2 \hat{x}_i \hat{x}_i^T \right) (\hat{X}^T \hat{X})^{-1} \right)$$

- Note that $\hat{u}_i = y_i - \mathbf{x}_i^T \hat{\beta}_{2SLS}$ (we use the true x_i not the predicted \hat{x}_i)

2SLS Procedures and Conditions for Multiple Endogenous Variables #flashcard

- Notations: L is the number of exogenous variables, K is the number of all variables in the equation of interest, $\underbrace{z_i^T}_{1 \times L}$ is a row vector of all exogenous variables (IVs and exogenous regressors), $\underbrace{x_i^T}_{1 \times K}$ is a row vector of all variables in the equation of interest
- 1st-stage Projection:

$$\underset{n \times K}{X} = \underset{n \times L}{Z} \underset{L \times K}{\Pi} + \underset{n \times K}{R}$$

note that if we have an intercept, we will always include an equation $1 = 1$ and if some variables x_k are exogenous, we need to include $x_k = x_k$

- Conditions:
 - Validity: $\mathbb{E}[z_i u_i] = 0$
 - Informative
 - Order condition (necessary but not sufficient): $L \geq K$
 - Rank condition (necessary and sufficient): the $L \times K$ matrix Π has full rank
- Then, calculate \hat{X} and run the main regression

Testing IV Validity in Over-identifying Cases #flashcard

- Idea: when we have over-identification ($L > K$), we can examine whether the minimised value of the GMM criterion function is "small enough" to be consistent with our orthogonal assumption $\mathbb{E}[z_i u_i] = 0$
- Conditional homoskedastic - **Sargan Test**
 - Sargan/J-test statistic:

$$J = \frac{1}{\hat{\sigma}^2} \hat{u}^T Z(Z^T Z)^{-1} Z^T \hat{u}$$

where $\hat{u}_i = y_i - x_i^T \hat{\beta}_{2SLS}$ and $\hat{\sigma}^2 = \frac{1}{n} \sum_{i=1}^n \hat{u}_i^2$

- Distribution under $H_0 : \mathbb{E}[z_i u_i] = 0$:

$$J \sim^a \chi_{L-K}^2$$

- Conditional heteroskedastic - **Hansen Test**
 - No detail description

Testing Endogeneity #flashcard

- We assume the IVs are valid and informative
- Idea: $\hat{\beta}_{OLS}$ and $\hat{\beta}_{2SLS}$ should be similar if the variable is exogenous
- Conditional homoskedastic - **Hausman Test**
 - Assumption:
 - Valid and informative IVs
 - Conditional homoskedasticity:

$$\mathbb{E}[u_i^2 | z_i] = \sigma^2$$

- The $K \times K$ matrix $(\widehat{Var}[\hat{\beta}_{2SLS}] - \widehat{Var}[\hat{\beta}_{OLS}])$ is non-singular
 - If this is singular, we can use the Moore-Penrose pseudo-inverse with rank R , and the distribution will be $h \sim^a \chi_R^2$
- $H_0 : \mathbb{E}[x_i u_i] = 0, H_1 : \mathbb{E}[x_i u_i] \neq 0$
- Test statistic:

$$h = (\hat{\beta}_{2SLS} - \hat{\beta}_{OLS})^T (\widehat{Var}[\hat{\beta}_{2SLS}] - \widehat{Var}[\hat{\beta}_{OLS}])^{-1} (\hat{\beta}_{2SLS} - \hat{\beta}_{OLS})$$

- Distribution under H_0 :

$$h \sim^a \chi_K^2$$

- If we are only interested in a **sub-vector** of β with K_1 variables, we simply repeat the above with our sub-vector, and the distribution will be $\chi_{K_1}^2$
- If we are only interested in **one parameter** β_k , then the test simplifies to:

$$h = \frac{(\hat{\beta}_{k,2SLS} - \hat{\beta}_{k,OLS})^2}{\widehat{Var}[\hat{\beta}_{k,2SLS}] - \widehat{Var}[\hat{\beta}_{k,OLS}]} \sim^a \chi_1^2$$

- Alternative method (can deal with heteroskedasticity easily): **Control Function Test**
 - Perform 2SLS estimation using the control function method
 - If there is only 1 endogenous variable of interest: use a t-test to test whether the coefficient on the 1st-stage residual is 0 in the 2nd-stage regression
 - If there are more than 1 endogenous variables of interest: use a Wald test to test whether all coefficients on the 1st-stage residual are jointly 0 in the 2nd-stage regression
 - We can easily deal with heteroskedasticity using HR estimator of variance, but testing on a sub-vector of β will be hard due to "generated regressors" problem.

Finite-Sample Problems #flashcard

- Overfitting: $\hat{\beta}_{2SLS} \rightarrow \hat{\beta}_{OLS}$ as $L \rightarrow n$
 - A simple way to investigate: calculate a sequence of 2SLS estimates based on smaller and smaller subsets of the original IVs, and check whether there's systematic tendency for $\hat{\beta}_{2SLS}$ to move away from $\hat{\beta}_{OLS}$

Weak Instruments #flashcard

- Finite sample bias + Large inconsistency

Tests for Weak Instruments #flashcard

- Run a Wald Test for the 1st stage: $H_0 : \delta_0 m = \delta_1 = \dots = \delta_M = 0$
- Test statistics $\sim F(M, n - L)$ and we typically require it to be greater than 10.

Weak IV Robust Inference: Anderson-Rubin Test #flashcard

- The Anderson-Rubin test is a robust test for the significance of endogenous regressors in IV models, and unlike the usual Wald or t-tests, it remains valid even when instruments are weak.
 - It tests the null hypothesis:

$$H_0 : \beta = \beta_0$$

where β is the coefficient on the endogenous regressor.

• Procedures

- We start with the model:

$$y = X\beta + \varepsilon$$

and instrument X using Z (with $\text{rank}(Z) = m$, number of instruments).

- Instead of relying on 2SLS estimates, the AR test does the following:

1. Move the hypothesized value to the left-hand side:

$$y - X\beta_0 = u$$

2. Test if the residual u is uncorrelated with the instruments Z :

$$H_0 : \mathbb{E}[Z^T u] = 0$$

3. Form the test statistic:

$$AR(\beta_0) = \frac{\hat{u}^T P_Z \hat{u}}{\hat{\sigma}^2}$$

where:

- $P_Z = Z(Z^T Z)^{-1} Z^T$ is the projection matrix onto the instrument space.

- $\hat{\sigma}^2$ is an estimator of the error variance (often from a reduced form).

4. Distribution under the null:

$$AR(\beta_0) \sim \chi_m^2$$

where m = number of instruments.

3 4 2 Local Average Treatment Effects

3 5 GMM

GMM Estimator #flashcard

- Setup:

$$y_i - x_i^T \beta = u_i(\beta), \quad \mathbb{E}[u_i] = 0, \quad \mathbb{E}[z_i u_i] = 0$$

- GMM Estimator:

$$\hat{\beta}_{GMM} = \arg \min_{\beta} \hat{u}^T Z W_n Z^T \hat{u}$$

- Expressions and Weak Consistency:

- Assumptions:

- $y_i = x_i^T \beta + u_i$

- (x_i, y_i, z_i) are iid

- $\text{Rank}(\mathbb{E}[z_i x_i^T]) = K$

- $W_n \xrightarrow{p} W$ is a symmetric and psd $L \times L$ matrix

- Then:

$$\hat{\beta}_{GMM} = \left((X^T Z) W_n (Z^T X) \right)^{-1} (X^T Z) W_n (Z^T y)$$

$\xrightarrow{p} \beta$

- and:

$$\sqrt{n}(\hat{\beta}_{GMM} - \beta) \xrightarrow{D} N(0, V)$$